Games/gameLib_fix/Conditioning_Symm.lean
@@ -1,0 +1,1501 @@
+/-
+Copyright (c) 2024 Yves Jäckle. All rights reserved.
+Released under Apache 2.0 license as described in the file LICENSE.
+Author: Yves Jäckle.
+-/
+
+import Games.gameLib_fix.Basic
+import Games.gameLib_fix.Termination
+
+
+-- # Conditioning
+
+
+def Symm_Game_World.world_after_fst {α β : Type u} (g : Symm_Game_World α β)
+  (fst_act : β) : Symm_Game_World α β := -- act not required to be legal
+  {g with init_game_state := g.transition g.init_game_state [] fst_act }
+
+
+@[simp]
+lemma Symm_Game_World.world_after_fst_init {α β : Type u} (g : Symm_Game_World α β)
+  (fst_act : β) : (g.world_after_fst fst_act).init_game_state = g.transition g.init_game_state [] fst_act :=
+  by rfl
+
+@[simp]
+lemma Symm_Game_World.world_after_fst_law {α β : Type u} (g : Symm_Game_World α β)
+  (fst_act : β) : (g.world_after_fst fst_act).law = g.law :=
+  by rfl
+
+
+@[simp]
+lemma Symm_Game_World.world_after_fst_win_states {α β : Type u} (g : Symm_Game_World α β)
+  (fst_act : β) : (g.world_after_fst fst_act).win_states = g.win_states :=
+  by rfl
+
+
+@[simp]
+lemma Symm_Game_World.world_after_fst_transition {α β : Type u} (g : Symm_Game_World α β)
+  (fst_act : β) : (g.world_after_fst fst_act).transition = g.transition :=
+  by rfl
+
+
+
+
+
+
+
+
+#exit
+
+
+-- # Easy termination
+
+
+inductive Symm_Game_World.has_WL (g : Symm_Game_World α β) : Prop where
+| wf : g.is_fst_win → g.has_WL
+| ws : g.is_snd_win → g.has_WL
+
+
+-- lemma Symm_Game_World.has_WL_init_end
+--   (g : Symm_Game_World α β)
+--   (hg : g.playable)
+--   (P : Prop)
+--   (hp : P)
+--   (h : (P ∧ (¬ g.win_states g.init_game_state)) → g.has_WL) :
+--   g.has_WL :=
+--   by
+--   obtain ⟨fs,ss,_,_⟩ := g.playable_has_strat hg
+--   by_cases q2 : g.win_states g.init_game_state
+--   · apply Symm_Game_World.has_WL.ws
+--     use fs
+--     intro _ _ _
+--     use 0
+--     constructor
+--     · decide
+--     · constructor
+--       · apply q2
+--       · intro t no
+--         contradiction
+--   · exact h ⟨hp, q2⟩
+
+
+
+
+
+-- # zSymm_Game
+
+structure zSymm_Game_World (α β : Type _) extends Symm_Game_World α β where
+  law_careless : careless toSymm_Game_World.law toSymm_Game_World.law toSymm_Game_World.init_game_state toSymm_Game_World.law toSymm_Game_World.transition
+  transition_careless : careless toSymm_Game_World.law toSymm_Game_World.law toSymm_Game_World.init_game_state toSymm_Game_World.transition toSymm_Game_World.transition
+  coherent : toSymm_Game_World.coherent_end
+  playable : toSymm_Game_World.playable
+
+
+
+structure zSymm_Game (α β : Type _) extends zSymm_Game_World α β where
+  /-- The first players strategy-/
+  fst_strat : Strategy α β
+  /-- The second players strategy-/
+  snd_strat : Strategy α β
+  /-- The first players strategy is legal wrt. `law` and the second strategy-/
+  fst_lawful : Strategy_legal_fst init_game_state law fst_strat snd_strat
+  /-- The second players strategy is legal wrt. `law` and the first strategy-/
+  snd_lawful : Strategy_legal_snd init_game_state law fst_strat snd_strat
+
+
+
+instance (l : List α): Decidable (l = []) :=
+  by
+  match l with
+  | [] => apply isTrue ; rfl
+  | x :: L => apply isFalse ; exact List.cons_ne_nil x L
+
+
+
+def fst_strat_deconditioned (s_strat : Strategy α β) (f_act : β) (g : Symm_Game_World α β) : Strategy α β :=
+  (fun _ hist => if hist = [] then f_act else s_strat (g.world_after_fst f_act).init_game_state (hist.dropLast))
+
+def snd_strat_deconditioned (f_strat : Strategy α β) (f_act : β) (g : Symm_Game_World α β) : Strategy α β :=
+  (fun _ hist => f_strat (g.world_after_fst f_act).init_game_state (hist.dropLast))
+
+
+lemma Symm_Game_World.History_of_deconditioned
+  (g: Symm_Game_World α β)
+  (fst_act: β)
+  (f_strat s_strat : Strategy α β)
+  (turn : ℕ):
+  let fst_strat := fst_strat_deconditioned s_strat fst_act g
+  let snd_strat := snd_strat_deconditioned f_strat fst_act g
+  History_on_turn g.init_game_state fst_strat snd_strat (turn + 1) =
+  (History_on_turn (g.world_after_fst fst_act).init_game_state f_strat s_strat turn) ++ [fst_act] :=
+  by
+  intro fst_strat snd_strat
+  induction' turn with t ih
+  · dsimp [History_on_turn, Turn_fst]
+    rw [if_pos (by decide), fst_strat_deconditioned, if_pos (by rfl)]
+  · dsimp only [History_on_turn] at *
+    by_cases q : Turn_fst (t+1)
+    · rw [Turn_fst_not_step] at q
+      rw [if_neg q] at *
+      rw [← Turn_fst_not_step] at q
+      rw [if_pos q, if_pos q] at *
+      rw [List.cons_append, ← ih]
+      congr
+      dsimp at ih
+      rw [← Symm_Game_World.world_after_fst_init] at ih
+      rw [ih]
+      rw [snd_strat_deconditioned, List.dropLast_concat]
+    · rw [if_neg q, if_neg q] at *
+      rw [Turn_fst_not_step, not_not] at q
+      rw [if_pos q] at *
+      rw [fst_strat_deconditioned, snd_strat_deconditioned, if_neg (by apply List.cons_ne_nil)]
+      rw [List.cons_append, ← ih]
+      congr
+      dsimp [snd_strat_deconditioned] at ih
+      rw [← Symm_Game_World.world_after_fst_init] at ih
+      rw [ih]
+      rw [List.dropLast_concat]
+
+
+def Symm_Game_World.transition_blind_fst (g : Symm_Game_World α β) : Prop :=
+  ∀ f_strat s_strat: Strategy α β, ∀ fst_act : β, g.law g.init_game_state [] fst_act →
+  let fst_strat := fst_strat_deconditioned s_strat fst_act g
+  let snd_strat := snd_strat_deconditioned f_strat fst_act g
+  ∀ turn : ℕ, ∀ act : β, g.transition (g.world_after_fst fst_act).init_game_state (History_on_turn (g.world_after_fst fst_act).init_game_state f_strat s_strat turn) act
+    = g.transition g.init_game_state (History_on_turn g.init_game_state fst_strat snd_strat (turn + 1)) act
+
+def Symm_Game_World.transition_blind_snd (g : Symm_Game_World α β) : Prop :=
+  ∀ f_strat s_strat: Strategy α β, ∀ fst_act : β, g.law g.init_game_state [] fst_act →
+  let fst_strat := fst_strat_deconditioned s_strat fst_act g
+  let snd_strat := snd_strat_deconditioned f_strat fst_act g
+  ∀ turn : ℕ, ∀ act : β, g.transition (g.world_after_fst fst_act).init_game_state (History_on_turn (g.world_after_fst fst_act).init_game_state f_strat s_strat turn) act
+    = g.transition g.init_game_state (History_on_turn g.init_game_state fst_strat snd_strat (turn + 1)) act
+
+
+def Symm_Game_World.transition_blind (g : Symm_Game_World α β) : Prop :=
+ g.transition_blind_fst ∧ g.transition_blind_snd
+
+
+def Symm_Game_World.strong_transition_blind_fst (g : Symm_Game_World α β) : Prop :=
+  ∀ fst_act : β, g.law g.init_game_state [] fst_act →
+  ∀ hist : List β, ∀ act : β, g.transition (g.world_after_fst fst_act).init_game_state hist act
+    = g.transition g.init_game_state (hist ++ [fst_act]) act
+
+def Symm_Game_World.strong_transition_blind_snd (g : Symm_Game_World α β) : Prop :=
+  ∀ fst_act : β, g.law g.init_game_state [] fst_act →
+  ∀ hist : List β, ∀ act : β, g.transition (g.world_after_fst fst_act).init_game_state hist act
+    = g.transition g.init_game_state (hist ++ [fst_act]) act
+
+
+def Symm_Game_World.strong_transition_blind (g : Symm_Game_World α β) : Prop :=
+ g.strong_transition_blind_fst ∧ g.strong_transition_blind_snd
+
+lemma Symm_Game_World.strong_transition_blind_toWeak (g : Symm_Game_World α β) :
+  g.strong_transition_blind → g.transition_blind :=
+  by
+  rintro ⟨f_strong, s_strong⟩
+  constructor
+  · intro f_strat s_strat f_act f_act_leg fst_strat snd_strat t act
+    rw [Symm_Game_World.History_of_deconditioned]
+    apply f_strong
+    exact f_act_leg
+  · intro f_strat s_strat f_act f_act_leg fst_strat snd_strat t act
+    rw [Symm_Game_World.History_of_deconditioned]
+    apply s_strong
+    exact f_act_leg
+
+
+def Symm_Game_World.world_after_preHist {α β : Type u} (g : Symm_Game_World α β)
+  (prehist : List β) : Symm_Game_World α β := -- act not required to be legal
+  match prehist with
+  | [] => g
+  | last :: L => {g with init_game_state := g.transition g.init_game_state L last}
+
+
+lemma Symm_Game_World.world_after_preHist_win_states {α β : Type u} (g : Symm_Game_World α β)
+  (prehist : List β) : (g.world_after_preHist prehist).win_states = g.win_states :=
+  by cases' prehist <;> rfl
+
+
+
+def Symm_Game_World.hyper_transition_blind_fst (g : Symm_Game_World α β) : Prop :=
+  ∀ prehist : List β, Hist_legal g.law g.law g.init_game_state prehist →
+  ∀ hist : List β, ∀ act : β, g.transition (g.world_after_preHist prehist).init_game_state hist act
+    = g.transition g.init_game_state (hist ++ prehist) act
+
+def Symm_Game_World.hyper_transition_blind_snd (g : Symm_Game_World α β) : Prop :=
+  ∀ prehist : List β, Hist_legal g.law g.law g.init_game_state prehist →
+  ∀ hist : List β, ∀ act : β, g.transition (g.world_after_preHist prehist).init_game_state hist act
+    = g.transition g.init_game_state (hist ++ prehist) act
+
+
+def Symm_Game_World.hyper_transition_blind (g : Symm_Game_World α β) : Prop :=
+ g.hyper_transition_blind_fst ∧ g.hyper_transition_blind_snd
+
+
+lemma Symm_Game_World.hyper_transition_blind_transition_eq (g : Symm_Game_World α β) :
+  g.hyper_transition_blind → (g.transition g.init_game_state = g.transition g.init_game_state) :=
+  by
+  intro h
+  have := h.2 [] (by apply Hist_legal.nil)
+  dsimp [Symm_Game_World.world_after_preHist] at this
+  simp_rw [List.append_nil] at this
+  rfl
+
+
+lemma Symm_Game_World.hyper_transition_blind_toStrong (g : Symm_Game_World α β) :
+  g.hyper_transition_blind → g.strong_transition_blind :=
+  by
+  rintro ⟨f_hyper, s_hyper⟩
+  constructor
+  · intro f_act f_leg hist act
+    specialize f_hyper [f_act] _ hist act
+    · apply Hist_legal.cons
+      · dsimp
+        rw [if_pos (by decide)]
+        exact f_leg
+      · apply Hist_legal.nil
+    · dsimp [Symm_Game_World.world_after_fst, Symm_Game_World.world_after_preHist] at *
+      exact f_hyper
+  · intro f_act f_leg hist act
+    specialize s_hyper [f_act] _ hist act
+    · apply Hist_legal.cons
+      · dsimp
+        rw [if_pos (by decide)]
+        exact f_leg
+      · apply Hist_legal.nil
+    · dsimp [Symm_Game_World.world_after_fst, Symm_Game_World.world_after_preHist] at *
+      exact s_hyper
+
+@[simp]
+lemma Symm_Game_World.world_after_preHist_singleton {α β : Type u} (g : Symm_Game_World α β)
+  (act : β) : g.world_after_preHist [act] = g.world_after_fst act :=
+  by
+  dsimp [Symm_Game_World.world_after_fst, Symm_Game_World.world_after_preHist]
+
+
+lemma zSymm_Game_World.is_hyper_transition_blind (g : zSymm_Game_World α β) :
+  g.toSymm_Game_World.hyper_transition_blind :=
+  by
+  constructor
+  · intro prehist preh_leg hist act
+    have := g.transition_careless g.init_game_state hist prehist
+    match prehist with
+    | [] =>
+        dsimp [Symm_Game_World.world_after_preHist]
+        rw [List.append_nil]
+    | x :: l =>
+        specialize this (by apply List.noConfusion)
+        rw [this]
+        · dsimp [Symm_Game_World.world_after_preHist]
+        · exact preh_leg
+  · intro prehist preh_leg hist act
+    have := g.transition_careless g.init_game_state hist prehist
+    match prehist with
+    | [] =>
+        dsimp [Symm_Game_World.world_after_preHist]
+        rw [List.append_nil]
+    | x :: l =>
+        specialize this (by apply List.noConfusion)
+        rw [this]
+        · dsimp [Symm_Game_World.world_after_preHist]
+        · exact preh_leg
+
+
+
+
+lemma Symm_Game_World.State_of_deconditioned
+  (g: Symm_Game_World α β)
+  (tb : g.transition_blind)
+  (fst_act: β)
+  (fst_act_legal: g.law g.init_game_state [] fst_act)
+  (f_strat s_strat : Strategy α β)
+  (turn : ℕ):
+  let fst_strat := fst_strat_deconditioned s_strat fst_act g
+  let snd_strat := snd_strat_deconditioned f_strat fst_act g
+  g.state_on_turn fst_strat snd_strat (turn + 1) =
+  (g.world_after_fst fst_act).state_on_turn f_strat s_strat turn :=
+  by
+  intro fst_strat snd_strat
+  cases' turn with t
+  · dsimp [state_on_turn]
+    rw [if_pos (by decide)]
+    dsimp [history_on_turn, History_on_turn]
+    rw [fst_strat_deconditioned, if_pos (by rfl)]
+  · dsimp [state_on_turn]
+    by_cases q : Turn_fst (t + 1)
+    · rw [if_pos q]
+      rw [Turn_fst_not_step] at q
+      rw [if_neg q]
+      dsimp [history_on_turn]
+      have := g.History_of_deconditioned fst_act f_strat s_strat t
+      dsimp at this
+      rw [this]
+      rw [snd_strat_deconditioned, List.dropLast_concat]
+      rw [← this]
+      clear this
+      have := tb.2 f_strat s_strat fst_act fst_act_legal
+      dsimp at this
+      specialize this t (f_strat (world_after_fst g fst_act).init_game_state (History_on_turn (world_after_fst g fst_act).init_game_state f_strat s_strat t))
+      rw [← Symm_Game_World.world_after_fst_init]
+      rw [← this]
+      clear this
+      rfl
+    · rw [Turn_not_fst_iff_snd, Turn_snd_fst_step] at q
+      rw [if_pos q]
+      dsimp [history_on_turn]
+      rw [← Turn_fst_step, Turn_fst_not_step] at q
+      rw [if_neg q]
+      rw [fst_strat_deconditioned, if_neg (by apply History_on_turn_nonempty_of_succ)]
+      have := g.History_of_deconditioned fst_act f_strat s_strat t
+      dsimp at this
+      rw [this]
+      rw [List.dropLast_concat]
+      rw [← this]
+      clear this
+      have := tb.1 f_strat s_strat fst_act fst_act_legal
+      dsimp at this
+      specialize this t (s_strat (world_after_fst g fst_act).init_game_state (History_on_turn (Symm_Game_World.transition g g.init_game_state [] fst_act) f_strat s_strat t))
+      rw [← Symm_Game_World.world_after_fst_init] at this
+      rw [← Symm_Game_World.world_after_fst_init]
+      rw [← this]
+
+
+lemma zSymm_Game_World.State_of_deconditioned
+  (g: zSymm_Game_World α β)
+  (fst_act: β)
+  (fst_act_legal: g.law g.init_game_state [] fst_act)
+  (f_strat s_strat : Strategy α β)
+  (turn : ℕ):
+  let fst_strat := fst_strat_deconditioned s_strat fst_act g.toSymm_Game_World
+  let snd_strat := snd_strat_deconditioned f_strat fst_act g.toSymm_Game_World
+  g.state_on_turn fst_strat snd_strat (turn + 1) =
+  (g.world_after_fst fst_act).state_on_turn f_strat s_strat turn :=
+  by
+  apply Symm_Game_World.State_of_deconditioned
+  · apply Symm_Game_World.strong_transition_blind_toWeak
+    apply Symm_Game_World.hyper_transition_blind_toStrong
+    apply zSymm_Game_World.is_hyper_transition_blind
+  · exact fst_act_legal
+
+
+
+
+
+
+
+-- -- # Careless strat
+
+
+-- def Game_World.Strategy_blind_fst (strat : Strategy α β) (g : Game_World α β) : Prop :=
+--   ∀ s_strat: Strategy α β,
+--   let fst_act := strat g.init_game_state []
+--   ∀ turn : ℕ, strat (g.world_after_fst fst_act).init_game_state (History_on_turn (g.world_after_fst fst_act).init_game_state s_strat strat turn)
+--     = strat g.init_game_state (History_on_turn g.init_game_state strat s_strat (turn + 1))
+
+
+-- def Game_World.Strategy_blind_snd (strat : Strategy α β) (g : Game_World α β) : Prop :=
+--   ∀ f_strat: Strategy α β,
+--   let fst_act := f_strat g.init_game_state []
+--   ∀ turn : ℕ, strat (g.world_after_fst fst_act).init_game_state (History_on_turn (g.world_after_fst fst_act).init_game_state strat f_strat turn)
+--     = strat g.init_game_state (History_on_turn g.init_game_state f_strat strat (turn + 1))
+
+-- def Game_World.Strategy_blind (strat : Strategy α β) (g : Game_World α β) : Prop :=
+--   g.Strategy_blind_fst strat ∧ g.Strategy_blind_snd strat
+
+-- def Game_World.strong_Strategy_blind (strat : Strategy α β) (g : Game_World α β) : Prop :=
+--   ∀ fst_act : β, g.law g.init_game_state [] fst_act →
+--   ∀ hist : List β, strat (g.world_after_fst fst_act).init_game_state hist
+--     = strat g.init_game_state (hist ++ [fst_act])
+
+-- lemma Game_World.world_after_fst_History_blind (g : Game_World α β)
+--   (f_strat s_strat : Strategy α β) (turn : ℕ)
+--   (hf : g.Strategy_blind_fst f_strat) (hs : g.Strategy_blind_snd s_strat)
+--   :
+--   (History_on_turn (g.world_after_fst (f_strat g.init_game_state [])).init_game_state s_strat f_strat turn)
+--   ++ [(f_strat g.init_game_state [])] = History_on_turn g.init_game_state f_strat s_strat (turn+1) :=
+--   by
+--   rw [History_on_turn]
+--   induction' turn with t ih
+--   · dsimp [History_on_turn]
+--     rw [if_pos (by decide)]
+--   · dsimp [History_on_turn]
+--     by_cases q : Turn_fst (t+1)
+--     · rw [if_pos q] at *
+--       rw [Turn_fst_not_step] at q
+--       rw [if_neg q]
+--       rw [← Turn_fst_not_step] at q
+--       rw [if_pos q]
+--       rw [Game_World.world_after_fst_init] at *
+--       rw [List.cons_append, ih]
+--       congr 1
+--       have := hs f_strat t
+--       rw [← Game_World.world_after_fst_init, this]
+--       dsimp [History_on_turn]
+--       rw [if_pos q]
+--     · rw [if_neg q] at *
+--       rw [Turn_fst_not_step, not_not] at q
+--       rw [if_pos q]
+--       rw [← @not_not (Turn_fst (t + 1 + 1)), ← Turn_fst_not_step] at q
+--       rw [if_neg q]
+--       rw [Game_World.world_after_fst_init] at *
+--       rw [List.cons_append]
+--       congr 1
+--       have := hf s_strat t
+--       rw [Game_World.world_after_fst_init] at this
+--       rw [this]
+--       dsimp [History_on_turn]
+--       rw [if_neg q]
+
+
+-- lemma Game_World.world_after_fst_History_strong_blind (g : Game_World α β)
+--   (f_strat s_strat : Strategy α β) (turn : ℕ)
+--   (f_leg : Strategy_legal_fst g.init_game_state g.law f_strat s_strat)
+--   (hf : g.strong_Strategy_blind f_strat) (hs : g.strong_Strategy_blind s_strat)
+--   :
+--   (History_on_turn (g.world_after_fst (f_strat g.init_game_state [])).init_game_state s_strat f_strat turn)
+--   ++ [(f_strat g.init_game_state [])] = History_on_turn g.init_game_state f_strat s_strat (turn+1) :=
+--   by
+--   rw [History_on_turn]
+--   induction' turn with t ih
+--   · dsimp [History_on_turn]
+--     rw [if_pos (by decide)]
+--   · unfold History_on_turn
+--     by_cases q : Turn_fst (t+1)
+--     · rw [if_pos q]
+--       rw [List.cons_append, ih]
+--       specialize hs (f_strat g.init_game_state []) (by apply f_leg 0 (by decide)) (History_on_turn (Game_World.transition g g.init_game_state [] (f_strat g.init_game_state [])) s_strat f_strat t)
+--       rw [← Game_World.world_after_fst_init] at hs
+--       rw [hs, ih]
+--       rw [if_neg (show ¬ Turn_fst (Nat.succ t + 1) from (by rw [← Turn_fst_not_step]; exact q))]
+--     · rw [if_neg q]
+--       rw [List.cons_append, ih]
+--       specialize hf (f_strat g.init_game_state []) (by apply f_leg 0 (by decide)) (History_on_turn (Game_World.transition g g.init_game_state [] (f_strat g.init_game_state [])) s_strat f_strat t)
+--       rw [← Game_World.world_after_fst_init] at hf
+--       rw [hf, ih]
+--       rw [if_pos (show Turn_fst (Nat.succ t + 1) from (by rw [iff_not_comm.mp (Turn_fst_not_step (t+1))]; exact q))]
+
+
+-- -- might not be the case, because we have no carelessness of other strat
+-- -- lemma Game_World.strong_Strategy_blind_toWeak (strat : Strategy α β) (g : Game_World α β)
+-- --   (f_leg : Strategy_legal_fst g.init_game_state g.law strat s_strat) :
+-- --   g.strong_Strategy_blind strat → g.Strategy_blind strat :=
+-- --   by
+-- --   intro hyp
+-- --   constructor
+-- --   · intro s_strat f_act t
+-- --     rw [hyp]
+
+
+
+-- --#exit
+
+-- def Game_World.hyper_Strategy_blind
+--   (strat : Strategy α β) (g : Game_World α β) : Prop :=
+--   ∀ prehist : List β, Hist_legal g.law g.law g.init_game_state prehist →
+--   ∀ hist : List β, strat (g.world_after_preHist prehist).init_game_state hist
+--     = strat g.init_game_state (hist ++ prehist)
+
+
+-- lemma Game_World.hyper_Strategy_blind_toStrong
+--   (strat : Strategy α β) (g : Game_World α β) :
+--   g.hyper_Strategy_blind strat → g.strong_Strategy_blind strat :=
+--   by
+--   intro hyp
+--   intro f_act f_leg hist
+--   specialize hyp [f_act] _ hist
+--   · apply Hist_legal.cons
+--     · dsimp
+--       rw [if_pos (by decide)]
+--       exact f_leg
+--     · apply Hist_legal.nil
+--   · dsimp [Game_World.world_after_fst, Game_World.world_after_preHist] at *
+--     exact hyp
+
+
+--#exit
+
+-- # Blind law
+
+def Symm_Game_World.legal_blind_fst (g : Symm_Game_World α β) : Prop :=
+  ∀ f_strat s_strat: Strategy α β, ∀ fst_act : β, g.law g.init_game_state [] fst_act →
+  let fst_strat := fst_strat_deconditioned s_strat fst_act g
+  let snd_strat := snd_strat_deconditioned f_strat fst_act g
+  ∀ turn : ℕ, ∀ act : β, g.law (g.world_after_fst fst_act).init_game_state (History_on_turn (g.world_after_fst fst_act).init_game_state f_strat s_strat turn) act
+    = g.law g.init_game_state (History_on_turn g.init_game_state fst_strat snd_strat (turn + 1)) act
+
+def Symm_Game_World.legal_blind_snd (g : Symm_Game_World α β) : Prop :=
+  ∀ f_strat s_strat: Strategy α β, ∀ fst_act : β, g.law g.init_game_state [] fst_act →
+  let fst_strat := fst_strat_deconditioned s_strat fst_act g
+  let snd_strat := snd_strat_deconditioned f_strat fst_act g
+  ∀ turn : ℕ, ∀ act : β, g.law (g.world_after_fst fst_act).init_game_state (History_on_turn (g.world_after_fst fst_act).init_game_state f_strat s_strat turn) act
+    = g.law g.init_game_state (History_on_turn g.init_game_state fst_strat snd_strat (turn + 1)) act
+
+
+def Symm_Game_World.legal_blind (g : Symm_Game_World α β) : Prop :=
+ g.legal_blind_fst ∧ g.legal_blind_snd
+
+
+def Symm_Game_World.strong_legal_blind_fst (g : Symm_Game_World α β) : Prop :=
+  ∀ fst_act : β, g.law g.init_game_state [] fst_act →
+  ∀ hist : List β, ∀ act : β, g.law (g.world_after_fst fst_act).init_game_state hist act
+    = g.law g.init_game_state (hist ++ [fst_act]) act
+
+def Symm_Game_World.strong_legal_blind_snd (g : Symm_Game_World α β) : Prop :=
+  ∀ fst_act : β, g.law g.init_game_state [] fst_act →
+  ∀ hist : List β, ∀ act : β, g.law (g.world_after_fst fst_act).init_game_state hist act
+    = g.law g.init_game_state (hist ++ [fst_act]) act
+
+
+def Symm_Game_World.strong_legal_blind (g : Symm_Game_World α β) : Prop :=
+ g.strong_legal_blind_fst ∧ g.strong_legal_blind_snd
+
+lemma Symm_Game_World.strong_legal_blind_toWeak (g : Symm_Game_World α β) :
+  g.strong_legal_blind → g.legal_blind :=
+  by
+  rintro ⟨f_strong, s_strong⟩
+  constructor
+  · intro f_strat s_strat f_act f_act_leg fst_strat snd_strat t act
+    rw [Symm_Game_World.History_of_deconditioned]
+    apply f_strong
+    exact f_act_leg
+  · intro f_strat s_strat f_act f_act_leg fst_strat snd_strat t act
+    rw [Symm_Game_World.History_of_deconditioned]
+    apply s_strong
+    exact f_act_leg
+
+
+
+
+def Symm_Game_World.hyper_legal_blind_fst (g : Symm_Game_World α β) : Prop :=
+  ∀ prehist : List β, Hist_legal g.law g.law g.init_game_state prehist →
+  ∀ hist : List β, ∀ act : β, g.law (g.world_after_preHist prehist).init_game_state hist act
+    = g.law g.init_game_state (hist ++ prehist) act
+
+def Symm_Game_World.hyper_legal_blind_snd (g : Symm_Game_World α β) : Prop :=
+  ∀ prehist : List β, Hist_legal g.law g.law g.init_game_state prehist →
+  ∀ hist : List β, ∀ act : β, g.law (g.world_after_preHist prehist).init_game_state hist act
+    = g.law g.init_game_state (hist ++ prehist) act
+
+
+def Symm_Game_World.hyper_legal_blind (g : Symm_Game_World α β) : Prop :=
+ g.hyper_legal_blind_fst ∧ g.hyper_legal_blind_snd
+
+
+lemma Symm_Game_World.hyper_legal_blind_legal_eq (g : Symm_Game_World α β) :
+  g.hyper_legal_blind → (g.law g.init_game_state = g.law g.init_game_state) :=
+  by
+  intro h
+  have := h.2 [] (by apply Hist_legal.nil)
+  dsimp [Symm_Game_World.world_after_preHist] at this
+  simp_rw [List.append_nil] at this
+  rfl
+
+
+lemma Symm_Game_World.hyper_legal_blind_toStrong (g : Symm_Game_World α β) :
+  g.hyper_legal_blind → g.strong_legal_blind :=
+  by
+  rintro ⟨f_hyper, s_hyper⟩
+  constructor
+  · intro f_act f_leg hist act
+    specialize f_hyper [f_act] _ hist act
+    · apply Hist_legal.cons
+      · dsimp
+        rw [if_pos (by decide)]
+        exact f_leg
+      · apply Hist_legal.nil
+    · dsimp [Symm_Game_World.world_after_fst, Symm_Game_World.world_after_preHist] at *
+      exact f_hyper
+  · intro f_act f_leg hist act
+    specialize s_hyper [f_act] _ hist act
+    · apply Hist_legal.cons
+      · dsimp
+        rw [if_pos (by decide)]
+        exact f_leg
+      · apply Hist_legal.nil
+    · dsimp [Symm_Game_World.world_after_fst, Symm_Game_World.world_after_preHist] at *
+      exact s_hyper
+
+
+lemma zSymm_Game_World.is_hyper_legal_blind (g : zSymm_Game_World α β) :
+  g.toSymm_Game_World.hyper_legal_blind :=
+  by
+  constructor
+  · intro prehist preh_leg hist act
+    have := g.law_careless g.init_game_state hist prehist
+    match prehist with
+    | [] =>
+        dsimp [Symm_Game_World.world_after_preHist]
+        rw [List.append_nil]
+    | x :: l =>
+        specialize this (by apply List.noConfusion)
+        rw [this]
+        · dsimp [Symm_Game_World.world_after_preHist]
+        · exact preh_leg
+  · intro prehist preh_leg hist act
+    have := g.law_careless g.init_game_state hist prehist
+    match prehist with
+    | [] =>
+        dsimp [Symm_Game_World.world_after_preHist]
+        rw [List.append_nil]
+    | x :: l =>
+        specialize this (by apply List.noConfusion)
+        rw [this]
+        · dsimp [Symm_Game_World.world_after_preHist]
+        · exact preh_leg
+
+
+lemma Symm_Game_World.law_deconditioned_fst
+  (g: Symm_Game_World α β)
+  (fst_act: β)
+  (fst_act_legal: g.law g.init_game_state [] fst_act)
+  (f_strat s_strat : Strategy α β)
+  (s_leg: Strategy_legal_snd (g.world_after_fst fst_act).init_game_state (g.world_after_fst fst_act).law f_strat s_strat)
+  (b : g.legal_blind_fst)
+  :
+  let fst_strat := fst_strat_deconditioned s_strat fst_act g
+  let snd_strat := snd_strat_deconditioned f_strat fst_act g
+  Strategy_legal_fst g.init_game_state g.law fst_strat snd_strat :=
+  by
+  intro fst_strat snd_strat t tf
+  cases' t with t
+  · dsimp [History_on_turn, fst_strat_deconditioned]
+    rw [if_pos (by rfl)]
+    exact fst_act_legal
+  · rw [← b, Symm_Game_World.History_of_deconditioned]
+    · dsimp [History_on_turn, fst_strat_deconditioned]
+      rw [if_neg (by apply List.append_ne_nil_of_ne_nil_right ; exact List.cons_ne_nil fst_act [])]
+      rw [List.dropLast_concat]
+      apply s_leg
+      rw [Turn_snd_fst_step]
+      exact tf
+    · exact fst_act_legal
+
+
+lemma Symm_Game_World.law_deconditioned_snd
+  (g: Symm_Game_World α β)
+  (fst_act: β)
+  (fst_act_legal: g.law g.init_game_state [] fst_act)
+  (f_strat s_strat : Strategy α β)
+  (f_leg: Strategy_legal_fst (g.world_after_fst fst_act).init_game_state (g.world_after_fst fst_act).law f_strat s_strat)
+  (b : g.legal_blind_snd)
+  :
+  let fst_strat := fst_strat_deconditioned s_strat fst_act g
+  let snd_strat := snd_strat_deconditioned f_strat fst_act g
+  Strategy_legal_snd g.init_game_state g.law fst_strat snd_strat :=
+  by
+  intro fst_strat snd_strat t tf
+  cases' t with t
+  · contradiction
+  · rw [← b, Symm_Game_World.History_of_deconditioned]
+    · dsimp [History_on_turn, snd_strat_deconditioned]
+      rw [List.dropLast_concat]
+      apply f_leg
+      rw [Turn_fst_snd_step]
+      exact tf
+    · exact fst_act_legal
+
+
+
+def zSymm_Game_World.world_after_fst {α β : Type u} (g : zSymm_Game_World α β)
+  (fst_act : β) (fst_act_legal: g.law g.init_game_state [] fst_act) : zSymm_Game_World α β :=
+  {(g.toSymm_Game_World.world_after_fst fst_act) with
+      law_careless := by dsimp ; apply g.law_careless
+      transition_careless := by dsimp ; apply g.transition_careless
+      coherent := by
+                  intro f_strat s_strat f_leg s_leg t
+                  intro fws
+                  dsimp at *
+                  have := g.State_of_deconditioned fst_act fst_act_legal f_strat s_strat
+                  dsimp [Symm_Game_World.world_after_fst] at this
+                  rw [← this] at *
+                  clear this
+                  have := (g.coherent (fst_strat_deconditioned s_strat fst_act g.toSymm_Game_World) (snd_strat_deconditioned f_strat fst_act g.toSymm_Game_World)
+                      (by apply g.law_deconditioned_fst fst_act fst_act_legal _ _ s_leg  (g.strong_legal_blind_toWeak (g.hyper_legal_blind_toStrong g.is_hyper_legal_blind)).1)
+                      (by apply g.law_deconditioned_snd fst_act fst_act_legal _ _ f_leg  (g.strong_legal_blind_toWeak (g.hyper_legal_blind_toStrong g.is_hyper_legal_blind)).2)
+                      (t+1))
+                  exact this fws
+      playable := by apply g.playable
+                  }
+
+
+
+lemma zSymm_Game_World.world_after_fst_init (g : zSymm_Game_World α β)
+  (fst_act : β) (fst_act_legal: g.law g.init_game_state [] fst_act) :
+  (g.world_after_fst fst_act fst_act_legal).init_game_state = g.transition g.init_game_state [] fst_act :=
+  by
+  rfl
+
+
+@[simp]
+lemma zSymm_Game_World.world_after_fst_law {α β : Type u} (g : zSymm_Game_World α β)
+  (fst_act : β) (fst_act_legal: g.law g.init_game_state [] fst_act) :
+  (g.world_after_fst fst_act fst_act_legal).law = g.law :=
+  by rfl
+
+
+@[simp]
+lemma zSymm_Game_World.world_after_fst_win_states {α β : Type u} (g : zSymm_Game_World α β)
+  (fst_act : β) (fst_act_legal: g.law g.init_game_state [] fst_act) :
+  (g.world_after_fst fst_act fst_act_legal).win_states = g.win_states :=
+  by rfl
+
+
+
+@[simp]
+lemma zSymm_Game_World.world_after_fst_transition {α β : Type u} (g : zSymm_Game_World α β)
+  (fst_act : β) (fst_act_legal: g.law g.init_game_state [] fst_act) :
+  (g.world_after_fst fst_act fst_act_legal).transition = g.transition :=
+  by rfl
+
+
+
+
+
+def zSymm_Game.history_on_turn {α β : Type u} (g : zSymm_Game α β) : ℕ → List β :=
+  History_on_turn g.init_game_state g.fst_strat g.snd_strat
+
+
+def zSymm_Game.state_on_turn {α β : Type u} (g : zSymm_Game α β) : ℕ → α
+| 0 => g.init_game_state
+| n+1 => let h := g.history_on_turn n
+         if Turn_fst (n+1)
+         then g.transition g.init_game_state h (g.fst_strat g.init_game_state h)
+         else g.transition g.init_game_state h (g.snd_strat g.init_game_state h)
+
+
+
+
+-- # Termination
+
+
+
+def zSymm_Game.fst_win  {α β : Type _} (g : zSymm_Game α β) : Prop :=
+  ∃ turn : ℕ, Turn_fst turn ∧ g.win_states (g.state_on_turn turn) ∧
+    (∀ t < turn, g.state_on_turn_neutral g.fst_strat g.snd_strat t)
+
+
+def zSymm_Game.snd_win  {α β : Type u} (g : zSymm_Game α β) : Prop :=
+  ∃ turn : ℕ, Turn_snd turn  ∧ g.win_states (g.state_on_turn turn) ∧
+    (∀ t < turn, g.state_on_turn_neutral g.fst_strat g.snd_strat t)
+
+
+
+def zSymm_Game_World.is_fst_win  {α β : Type u} (g : zSymm_Game_World α β) : Prop :=
+  ∃ ws : Strategy α β, --g.Strategy_blind_fst ws ∧
+  ∀ snd_s : Strategy α β, --g.Strategy_blind_fst snd_s →
+   (snd_leg : Strategy_legal_snd g.init_game_state g.law ws snd_s) →
+   ∃ (ws_leg : Strategy_legal_fst g.init_game_state g.law ws snd_s),
+  ({g with fst_strat := ws, fst_lawful := ws_leg, snd_strat := snd_s, snd_lawful := snd_leg} : Symm_Game α β).fst_win
+
+
+def zSymm_Game_World.is_snd_win  {α β : Type u} (g : zSymm_Game_World α β) : Prop :=
+  ∃ ws : Strategy α β, -- g.Strategy_blind_snd ws ∧
+  ∀ fst_s : Strategy α β, --g.Strategy_blind_snd fst_s →
+   (fst_leg : Strategy_legal_fst g.init_game_state g.law fst_s ws) →
+   ∃ (ws_leg : Strategy_legal_snd g.init_game_state g.law fst_s ws),
+  ({g with fst_strat := fst_s, fst_lawful := fst_leg, snd_strat := ws, snd_lawful := ws_leg} : Symm_Game α β).snd_win
+
+
+
+inductive zSymm_Game_World.has_WL (g : zSymm_Game_World α β) : Prop where
+| wf : g.is_fst_win → g.has_WL
+| ws : g.is_snd_win → g.has_WL
+
+
+lemma zSymm_Game_World.has_WL_init_end
+  [Inhabited β ]
+  (g : zSymm_Game_World α β)
+  (P : Prop)
+  (hp : P)
+  (h : (P ∧ (¬ g.win_states g.init_game_state)) → g.has_WL) :
+  g.has_WL :=
+  by
+  --obtain ⟨ss,ss_prop⟩ := g.playable_has_strong_snd_strat g.playable
+
+  by_cases q2 : g.win_states g.init_game_state
+  · apply zSymm_Game_World.has_WL.ws
+    use (exStrat g.law g.playable)
+    intro fs fs_leg
+    constructor
+    · use 0
+      constructor
+      · decide
+      · constructor
+        · apply q2
+        · intro t no
+          contradiction
+    · exact (g.toSymm_Game_World.playable_has_strong_snd_strat g.playable) fs fs_leg
+  · exact h ⟨hp, q2⟩
+
+
+-- --#exit
+
+
+-- lemma zSymm_Game_World.has_WL_init_end
+--   (g : zSymm_Game_World α β)
+--   (P : Prop)
+--   (hp : P)
+--   (h : (P ∧ (¬ g.win_states g.init_game_state)) → g.has_WL) :
+--   g.has_WL :=
+--   by
+--   obtain ⟨ss,ss_prop⟩ := g.playable_has_strong_snd_strat g.playable
+--   by_cases q2 : g.win_states g.init_game_state
+--   · apply zSymm_Game_World.has_WL.ws
+--     use ss
+--     intro fs fs_leg
+--     constructor
+--     · use 0
+--       constructor
+--       · decide
+--       · constructor
+--         · apply q2
+--         · intro t no
+--           contradiction
+--     · exact ss_prop fs fs_leg
+--   · exact h ⟨hp, q2⟩
+
+--#exit
+
+-- # More conditioining
+
+def zSymm_Game_World.snd_strat_conditioned (f_strat : Strategy α β) (f_act : β) (g : zSymm_Game_World α β) : Strategy α β :=
+  fun _ hist => f_strat g.init_game_state (hist ++ [f_act])
+
+open Classical
+
+noncomputable
+def zSymm_Game_World.fst_strat_conditioned [Inhabited β] (g : zSymm_Game_World α β)
+  (f_strat : (h : List β) → (hne : h ≠ []) → (hl : g.law g.init_game_state [] (h.getLast hne)) → Strategy α β)
+  : Strategy α β :=
+  fun (_ : α) hist  =>
+    if hh : hist = [] -- shouldn't happen, as snd strat
+    then default -- dummy
+    else let f_act := List.getLast hist hh
+         if H : g.law g.init_game_state [] f_act-- should be the cases ?!?
+         then (f_strat hist hh H) (g.transition g.init_game_state [] f_act) hist.dropLast -- is it ? since ref to history in current game
+         else default
+
+
+lemma zSymm_Game_World.fst_strat_conditioned_get_rw_to_work [Inhabited β] (g : zSymm_Game_World α β)
+  (f_strat : (h : List β) → (hne : h ≠ []) → (hl : g.law g.init_game_state [] (h.getLast hne)) → Strategy α β) :
+  g.fst_strat_conditioned f_strat =
+  fun (_ : α) hist  =>
+    if hh : hist = [] -- shouldn't happen, as snd strat
+    then default -- dummy
+    else let f_act := List.getLast hist hh
+         if H : g.law g.init_game_state [] f_act-- should be the cases ?!?
+         then (f_strat hist hh H) (g.transition g.init_game_state [] f_act) hist.dropLast -- is it ? since ref to history in current game
+         else default
+  :=
+  by
+  rfl
+
+
+
+
+lemma zSymm_Game_World.history_on_turn_conditioned
+  [Inhabited β] (g : zSymm_Game_World α β) (fst_s: Strategy α β)
+  (f_strat : (h : List β) → (hne : h ≠ []) → (hl : g.law g.init_game_state [] (h.getLast hne)) → Strategy α β)
+  (h_f_strat : ∀ h H: List β, (hne : h ≠ []) → (Hne : H ≠ []) →
+      (hl : g.law g.init_game_state [] (h.getLast hne)) → (Hl : g.law g.init_game_state [] (H.getLast Hne)) →
+      h.getLast hne = H.getLast Hne →
+      f_strat h hne hl = f_strat H Hne Hl)
+  (f_act_leg : g.law g.init_game_state [] (fst_s g.init_game_state [])):
+  let f_act := fst_s g.init_game_state []
+  ∀ t : ℕ,
+  g.history_on_turn fst_s (g.fst_strat_conditioned f_strat) (t+1) =
+  ((g.world_after_fst f_act f_act_leg).history_on_turn (f_strat [f_act] (List.cons_ne_nil f_act []) f_act_leg) (g.snd_strat_conditioned fst_s f_act) t) ++ [f_act]:=
+  by
+  intro f_act t
+  induction' t with t ih
+  · dsimp [Symm_Game_World.history_on_turn, History_on_turn]
+    rw [if_pos (by decide)]
+  · dsimp [Symm_Game_World.history_on_turn, History_on_turn]
+    by_cases q : Turn_fst (Nat.succ t + 1)
+    · rw [if_pos q]
+      rw [iff_not_comm.mp (Turn_fst_not_step (t+1))] at q
+      rw [if_neg q,if_neg q]
+      dsimp [zSymm_Game_World.snd_strat_conditioned]
+      unfold Symm_Game_World.history_on_turn at ih
+      rw [← ih]
+      dsimp [History_on_turn]
+      rw [if_neg q]
+    · rw [if_neg q]
+      rw [iff_not_comm.mp (Turn_fst_not_step (t+1)), not_not] at q
+      rw [if_pos q, if_pos q]
+      dsimp [zSymm_Game_World.fst_strat_conditioned]
+      rw [dif_neg (by apply List.cons_ne_nil)]
+      have := History_on_turn_getLast_fst_act g.init_game_state fst_s (g.fst_strat_conditioned f_strat) (t)
+      dsimp [History_on_turn] at this
+      simp_rw [if_pos q] at this
+      rw [dif_pos (by rw [this] ; apply f_act_leg)]
+      unfold Symm_Game_World.history_on_turn at ih
+      rw [← ih]
+      have that : History_on_turn g.init_game_state fst_s (fst_strat_conditioned g f_strat) (t + 1) =
+                  (fst_s g.init_game_state (History_on_turn g.init_game_state fst_s (fst_strat_conditioned g f_strat) t) ::
+                   History_on_turn g.init_game_state fst_s (fst_strat_conditioned g f_strat) t) :=
+        by
+        dsimp [History_on_turn]
+        rw [if_pos q]
+      have thut : List.getLast (History_on_turn g.init_game_state fst_s (g.fst_strat_conditioned f_strat) (t + 1))  (by apply History_on_turn_nonempty_of_succ) = f_act :=
+        by
+        simp_rw [ih]
+        rw [List.getLast_append]
+      simp_rw [← that]
+      specialize h_f_strat (History_on_turn g.init_game_state fst_s (g.fst_strat_conditioned f_strat) (t + 1)) [f_act]
+                  (by apply History_on_turn_nonempty_of_succ) (by apply List.cons_ne_nil)
+                  (by rw [thut] ; apply f_act_leg) (by apply f_act_leg)
+                  (by apply thut)
+      rw [h_f_strat]
+      congr
+      rw [ih]
+      rw [List.dropLast_append_of_ne_nil _ (show [f_act] ≠ [] from by apply List.cons_ne_nil)]
+      dsimp
+      rw [List.append_nil]
+
+
+
+
+
+lemma zSymm_Game_World.state_on_turn_conditioned
+  [Inhabited β] (g : zSymm_Game_World α β) (fst_s: Strategy α β)
+  (f_strat : (h : List β) → (hne : h ≠ []) → (hl : g.law g.init_game_state [] (h.getLast hne)) → Strategy α β)
+  (h_f_strat : ∀ h H: List β, (hne : h ≠ []) → (Hne : H ≠ []) →
+      (hl : g.law g.init_game_state [] (h.getLast hne)) → (Hl : g.law g.init_game_state [] (H.getLast Hne)) →
+      h.getLast hne = H.getLast Hne →
+      f_strat h hne hl = f_strat H Hne Hl)
+  (f_act_leg : g.law g.init_game_state [] (fst_s g.init_game_state [])):
+  let f_act := fst_s g.init_game_state []
+  ∀ t : ℕ,
+  g.state_on_turn fst_s (g.fst_strat_conditioned f_strat) (t+1) =
+  (g.world_after_fst f_act f_act_leg).state_on_turn (f_strat [f_act] (List.cons_ne_nil f_act []) f_act_leg) (g.snd_strat_conditioned fst_s f_act) t:=
+  by
+  intro f_act t
+  cases' t with t
+  · dsimp [Symm_Game_World.state_on_turn]
+    rw [if_pos (by decide)]
+    dsimp [Symm_Game_World.history_on_turn, History_on_turn, zSymm_Game_World.world_after_fst_init]
+  · dsimp [Symm_Game_World.state_on_turn]
+    by_cases q : Turn_fst (t + 1 + 1)
+    · rw [if_pos q]
+      rw [iff_not_comm.mp (Turn_fst_not_step (t+1))] at q
+      rw [if_neg q]
+      rw [g.history_on_turn_conditioned fst_s f_strat h_f_strat f_act_leg]
+      have := careless_singleton _ _ _ _ _ (g.transition_careless)
+      specialize this g.init_game_state ((Symm_Game_World.history_on_turn (world_after_fst g (fst_s g.init_game_state []) f_act_leg).toSymm_Game_World
+          (f_strat [fst_s g.init_game_state []] ((by apply List.cons_ne_nil) : [fst_s g.init_game_state []] ≠ []) f_act_leg)
+          (snd_strat_conditioned fst_s (fst_s g.init_game_state []) g) t)) f_act f_act_leg
+      simp_rw [this]
+      congr
+    · rw [if_neg q]
+      rw [iff_not_comm.mp (Turn_fst_not_step (t+1)), not_not] at q
+      rw [if_pos q]
+      rw [g.history_on_turn_conditioned fst_s f_strat h_f_strat f_act_leg]
+      have := careless_singleton _ _ _ _ _ (g.transition_careless)
+      specialize this g.init_game_state ((Symm_Game_World.history_on_turn (world_after_fst g (fst_s g.init_game_state []) f_act_leg).toSymm_Game_World
+          (f_strat [fst_s g.init_game_state []] ((by apply List.cons_ne_nil) : [fst_s g.init_game_state []] ≠ []) f_act_leg)
+          (snd_strat_conditioned fst_s (fst_s g.init_game_state []) g) t)) f_act f_act_leg
+      simp_rw [this]
+      congr
+      dsimp [fst_strat_conditioned]
+      rw [dif_neg (by apply List.append_ne_nil_of_ne_nil_right ; apply List.cons_ne_nil)]
+      rw [dif_pos (by rw [List.getLast_append] ; apply f_act_leg)]
+      rw [List.dropLast_append_of_ne_nil _ (show [f_act] ≠ [] from by apply List.cons_ne_nil)]
+      dsimp
+      rw [List.append_nil]
+      have := h_f_strat ((Symm_Game_World.history_on_turn (world_after_fst g (fst_s g.init_game_state []) f_act_leg).toSymm_Game_World
+            (f_strat [fst_s g.init_game_state []] ((by apply List.cons_ne_nil) : [fst_s g.init_game_state []] ≠ []) f_act_leg)
+            (snd_strat_conditioned fst_s (fst_s g.init_game_state []) g) t ++
+             [fst_s g.init_game_state []])) [f_act]
+             (by apply List.append_ne_nil_of_ne_nil_right ; apply List.cons_ne_nil)
+             (by apply List.cons_ne_nil)
+             (by rw [List.getLast_append] ; apply f_act_leg)
+             (by apply f_act_leg)
+             (by rw [List.getLast_append] ; dsimp)
+      rw [this]
+      rw [List.getLast_append]
+      rfl
+
+
+
+lemma zSymm_Game_World.conditioned_legal_fst
+  [Inhabited β] (g : zSymm_Game_World α β) (fst_s: Strategy α β)
+  (f_strat : (h : List β) → (hne : h ≠ []) → (hl : g.law g.init_game_state [] (h.getLast hne)) → Strategy α β)
+  (h_f_strat : ∀ h H: List β, (hne : h ≠ []) → (Hne : H ≠ []) →
+      (hl : g.law g.init_game_state [] (h.getLast hne)) → (Hl : g.law g.init_game_state [] (H.getLast Hne)) →
+      h.getLast hne = H.getLast Hne →
+      f_strat h hne hl = f_strat H Hne Hl)
+  (f_act_leg : g.law g.init_game_state [] (fst_s g.init_game_state [])) :
+  let f_act := fst_s g.init_game_state []
+  Strategy_legal_fst g.init_game_state g.law fst_s (g.fst_strat_conditioned f_strat)
+  ↔ Strategy_legal_snd (g.world_after_fst f_act f_act_leg).init_game_state (g.world_after_fst f_act f_act_leg).law (f_strat [f_act] (List.cons_ne_nil f_act []) f_act_leg) (g.snd_strat_conditioned fst_s f_act) :=
+  by
+  intro f_act
+  constructor
+  · intro leg t ts
+    have hh := g.history_on_turn_conditioned fst_s f_strat h_f_strat f_act_leg t
+    have hc := careless_singleton _ _ _ _ _ (g.law_careless)
+    specialize leg (t+1) (by rw [← Turn_snd_fst_step] ; exact ts)
+    unfold Symm_Game_World.history_on_turn at hh
+    rw [hh] at leg
+    rw [hc] at leg
+    · dsimp [snd_strat_conditioned]
+      apply leg
+    · apply f_act_leg
+  · intro leg t tf
+    cases' t with t
+    · dsimp [History_on_turn]
+      apply f_act_leg
+    · specialize leg (t) (by rw [Turn_snd_fst_step] ; exact tf)
+      have hh := g.history_on_turn_conditioned fst_s f_strat h_f_strat f_act_leg t
+      have hc := careless_singleton _ _ _ _ _ (g.law_careless)
+      unfold Symm_Game_World.history_on_turn at hh
+      rw [hh, hc]
+      · dsimp [snd_strat_conditioned] at leg
+        apply leg
+      · apply f_act_leg
+
+
+
+
+lemma zSymm_Game_World.conditioned_legal_snd
+  [Inhabited β] (g : zSymm_Game_World α β) (fst_s: Strategy α β)
+  (f_strat : (h : List β) → (hne : h ≠ []) → (hl : g.law g.init_game_state [] (h.getLast hne)) → Strategy α β)
+  (h_f_strat : ∀ h H: List β, (hne : h ≠ []) → (Hne : H ≠ []) →
+      (hl : g.law g.init_game_state [] (h.getLast hne)) → (Hl : g.law g.init_game_state [] (H.getLast Hne)) →
+      h.getLast hne = H.getLast Hne →
+      f_strat h hne hl = f_strat H Hne Hl)
+  (f_act_leg : g.law g.init_game_state [] (fst_s g.init_game_state [])) :
+  let f_act := fst_s g.init_game_state []
+  Strategy_legal_snd g.init_game_state g.law fst_s (g.fst_strat_conditioned f_strat)
+  ↔ Strategy_legal_fst (g.world_after_fst f_act f_act_leg).init_game_state (g.world_after_fst f_act f_act_leg).law (f_strat [f_act] (List.cons_ne_nil f_act []) f_act_leg) (g.snd_strat_conditioned fst_s f_act) :=
+  by
+  intro f_act
+  constructor
+  · intro leg t tf
+    have hh := g.history_on_turn_conditioned fst_s f_strat h_f_strat f_act_leg t
+    have hc := careless_singleton _ _ _ _ _ (g.law_careless)
+    specialize leg (t+1) (by rw [← Turn_fst_snd_step] ; exact tf)
+    unfold Symm_Game_World.history_on_turn at hh
+    rw [hh] at leg
+    rw [hc] at leg
+    · dsimp [snd_strat_conditioned]
+      dsimp [fst_strat_conditioned] at leg
+      rw [dif_neg (by apply List.append_ne_nil_of_ne_nil_right ; apply List.cons_ne_nil)] at leg
+      rw [dif_pos (by rw [List.getLast_append] ; apply f_act_leg)] at leg
+      rw [List.dropLast_append_of_ne_nil _ (show [f_act] ≠ [] from by apply List.cons_ne_nil)] at leg
+      dsimp at leg
+      rw [List.append_nil] at leg
+      have := h_f_strat ((Symm_Game_World.history_on_turn (world_after_fst g (fst_s g.init_game_state []) f_act_leg).toSymm_Game_World
+              (f_strat [fst_s g.init_game_state []] ((by apply List.cons_ne_nil) : [fst_s g.init_game_state []] ≠ []) f_act_leg)
+              (snd_strat_conditioned fst_s (fst_s g.init_game_state []) g) t ++
+              [fst_s g.init_game_state []])) [f_act]
+              (by apply List.append_ne_nil_of_ne_nil_right ; apply List.cons_ne_nil)
+              (by apply List.cons_ne_nil)
+              (by rw [List.getLast_append] ; apply f_act_leg)
+              (by apply f_act_leg)
+              (by rw [List.getLast_append] ; dsimp)
+      unfold Symm_Game_World.history_on_turn at this
+      rw [this] at leg
+      rw [List.getLast_append] at leg
+      apply leg
+    · apply f_act_leg
+  · intro leg t ts
+    cases' t with t
+    · contradiction
+    · have hh := g.history_on_turn_conditioned fst_s f_strat h_f_strat f_act_leg t
+      have hc := careless_singleton _ _ _ _ _ (g.law_careless)
+      specialize leg (t) (by rw [Turn_fst_snd_step] ; exact ts)
+      unfold Symm_Game_World.history_on_turn at hh
+      rw [hh]
+      rw [hc]
+      · rw [zSymm_Game_World.world_after_fst_law] at leg
+        convert leg using 1
+        dsimp [fst_strat_conditioned]
+        rw [dif_neg (by apply List.append_ne_nil_of_ne_nil_right ; apply List.cons_ne_nil)]
+        rw [dif_pos (by rw [List.getLast_append] ; apply f_act_leg)]
+        rw [List.dropLast_append_of_ne_nil _ (show [f_act] ≠ [] from by apply List.cons_ne_nil)]
+        dsimp
+        rw [List.append_nil]
+        have := h_f_strat ((Symm_Game_World.history_on_turn (world_after_fst g (fst_s g.init_game_state []) f_act_leg).toSymm_Game_World
+                (f_strat [fst_s g.init_game_state []] ((by apply List.cons_ne_nil) : [fst_s g.init_game_state []] ≠ []) f_act_leg)
+                (snd_strat_conditioned fst_s (fst_s g.init_game_state []) g) t ++
+                [fst_s g.init_game_state []])) [f_act]
+                (by apply List.append_ne_nil_of_ne_nil_right ; apply List.cons_ne_nil)
+                (by apply List.cons_ne_nil)
+                (by rw [List.getLast_append] ; apply f_act_leg)
+                (by apply f_act_leg)
+                (by rw [List.getLast_append] ; dsimp)
+        unfold Symm_Game_World.history_on_turn at this
+        rw [this]
+        rw [List.getLast_append]
+        rfl
+      · apply f_act_leg
+
+
+
+lemma zSymm_Game_World.conditioned_state_on_turn_neutral
+  [Inhabited β] (g : zSymm_Game_World α β) (fst_s: Strategy α β)
+  (f_strat : (h : List β) → (hne : h ≠ []) → (hl : g.law g.init_game_state [] (h.getLast hne)) → Strategy α β)
+  (h_f_strat : ∀ h H: List β, (hne : h ≠ []) → (Hne : H ≠ []) →
+      (hl : g.law g.init_game_state [] (h.getLast hne)) → (Hl : g.law g.init_game_state [] (H.getLast Hne)) →
+      h.getLast hne = H.getLast Hne →
+      f_strat h hne hl = f_strat H Hne Hl)
+  (f_act_leg : g.law g.init_game_state [] (fst_s g.init_game_state [])):
+  let f_act := fst_s g.init_game_state []
+  ∀ t : ℕ,
+  g.state_on_turn_neutral fst_s (g.fst_strat_conditioned f_strat) (t+1) =
+  (g.world_after_fst f_act f_act_leg).state_on_turn_neutral (f_strat [f_act] (List.cons_ne_nil f_act []) f_act_leg) (g.snd_strat_conditioned fst_s f_act) t:=
+  by
+  intro f_act t
+  dsimp [Symm_Game_World.state_on_turn_neutral]
+  rw [g.state_on_turn_conditioned fst_s f_strat h_f_strat f_act_leg]
+  by_cases q : Turn_fst t
+  · rw [if_pos q]
+    rw [Turn_fst_not_step] at q
+    rw [if_neg q]
+  · rw [if_neg q]
+    rw [Turn_fst_not_step, not_not] at q
+    rw [if_pos q]
+
+
+
+
+lemma History_on_turn_eq_strats_snd
+  (g : zSymm_Game_World α β) (f_strat sSa aSb: Strategy α β)
+  (h : ∀ t, Turn_snd (t+1) →  sSa g.init_game_state (History_on_turn g.init_game_state f_strat sSa (t)) =
+          sSb g.init_game_state (History_on_turn g.init_game_state f_strat sSb (t))) :
+  History_on_turn g.init_game_state f_strat sSa = History_on_turn g.init_game_state f_strat sSb :=
+  by
+  funext t
+  induction' t with t ih
+  · dsimp [History_on_turn]
+  · dsimp [History_on_turn]
+    by_cases q : Turn_fst (t + 1)
+    · rw [if_pos q, if_pos q, ih]
+    · specialize h t (by rw [Turn_not_fst_iff_snd] at q ; exact q)
+      rw [if_neg q, if_neg q, h, ih]
+
+
+lemma Strategy_legal_fst_eq_strats_snd
+  (g : zSymm_Game_World α β) (f_strat sSa sSb: Strategy α β)
+  (h : ∀ t, Turn_snd (t+1) → sSa g.init_game_state (History_on_turn g.init_game_state f_strat sSa (t)) =
+          sSb g.init_game_state (History_on_turn g.init_game_state f_strat sSb (t)))
+  (hl : Strategy_legal_fst g.init_game_state g.law f_strat sSa) :
+  Strategy_legal_fst g.init_game_state g.law f_strat sSb :=
+  by
+  intro t tf
+  rw [← History_on_turn_eq_strats_snd g f_strat sSa sSb h]
+  exact hl t tf
+
+
+lemma Strategy_legal_snd_eq_strats_snd
+  (g : zSymm_Game_World α β) (f_strat sSa sSb: Strategy α β)
+  (h : ∀ t, Turn_snd (t+1) → sSa g.init_game_state (History_on_turn g.init_game_state f_strat sSa (t)) =
+          sSb g.init_game_state (History_on_turn g.init_game_state f_strat sSb (t)))
+  (hl : Strategy_legal_snd g.init_game_state g.law f_strat sSa) :
+  Strategy_legal_snd g.init_game_state g.law f_strat sSb :=
+  by
+  intro t ts
+  rw [← History_on_turn_eq_strats_snd g f_strat sSa sSb h]
+  specialize hl t ts
+  rw [h t ts, ← History_on_turn_eq_strats_snd g f_strat sSa sSb h] at hl
+  exact hl
+
+
+
+lemma Conditioning_win [Inhabited β] (g : zSymm_Game_World α β) (fst_s: Strategy α β)
+  (f_strat : (h : List β) → (hne : h ≠ []) → (hl : g.law g.init_game_state [] (h.getLast hne)) → Strategy α β)
+  (h_f_strat : ∀ h H: List β, (hne : h ≠ []) → (Hne : H ≠ []) →
+      (hl : g.law g.init_game_state [] (h.getLast hne)) → (Hl : g.law g.init_game_state [] (H.getLast Hne)) →
+      h.getLast hne = H.getLast Hne →
+      f_strat h hne hl = f_strat H Hne Hl)
+  (f_act_leg : g.law g.init_game_state [] (fst_s g.init_game_state []))
+  (Leg_f : Strategy_legal_fst g.init_game_state g.law fst_s (zSymm_Game_World.fst_strat_conditioned g f_strat))
+  (Leg_s : Strategy_legal_snd g.init_game_state g.law fst_s (zSymm_Game_World.fst_strat_conditioned g f_strat))
+  (wlg_ws : ¬Symm_Game_World.win_states g.toSymm_Game_World g.init_game_state)
+  (hw : let f_act := fst_s g.init_game_state []
+        Symm_Game.fst_win { toSymm_Game_World := (g.world_after_fst f_act f_act_leg).toSymm_Game_World,
+                              fst_strat := f_strat [f_act] (by apply List.cons_ne_nil) f_act_leg,
+                              snd_strat := g.snd_strat_conditioned fst_s f_act,
+                              fst_lawful :=
+                                (by
+                                have := g.conditioned_legal_snd fst_s f_strat h_f_strat f_act_leg
+                                dsimp at this
+                                rw [zSymm_Game_World.world_after_fst_law, ← this]
+                                exact Leg_s),
+                              snd_lawful :=
+                                (by
+                                have := g.conditioned_legal_fst fst_s f_strat h_f_strat f_act_leg
+                                dsimp at this
+                                rw [zSymm_Game_World.world_after_fst_law, ← this]
+                                exact Leg_f),
+                                }) :
+    Symm_Game.snd_win { toSymm_Game_World := g.toSymm_Game_World,
+                          fst_strat := fst_s,
+                          snd_strat := (zSymm_Game_World.fst_strat_conditioned g f_strat),
+                          fst_lawful := (Leg_f),
+                          snd_lawful := (Leg_s)} :=
+  by
+  obtain ⟨t, ⟨ts,tw,tn⟩⟩ := hw
+  use (t+1)
+  constructor
+  · rw [← Turn_fst_snd_step]
+    exact ts
+  · constructor
+    · dsimp at tw
+      convert tw using 1
+      apply g.state_on_turn_conditioned fst_s f_strat h_f_strat f_act_leg
+    · intro n nt
+      cases' n with n
+      · dsimp [Symm_Game.state_on_turn_neutral]
+        rw [if_neg (by decide)]
+        dsimp [Symm_Game.state_on_turn]
+        exact wlg_ws
+      · have := g.conditioned_state_on_turn_neutral fst_s f_strat h_f_strat f_act_leg n
+        apply Symm_Game.state_on_turn_neutral_from_World _ (n+1)
+        dsimp
+        rw [this]
+        apply tn
+        exact Nat.lt_of_add_lt_add_right nt
+
+
+-- # Even more conditioining
+
+def zSymm_Game_World.snd_strat_reconditioned (s_strat : Strategy α β) (f_act : β) (g : zSymm_Game_World α β) (f_act_leg : g.law g.init_game_state [] f_act) : Strategy α β :=
+  fun _ hist => if hist = [] then f_act else s_strat (g.world_after_fst f_act f_act_leg).init_game_state (hist.dropLast)
+
+def zSymm_Game_World.fst_strat_reconditioned (f_strat : Strategy α β) (f_act : β) (g : zSymm_Game_World α β) : Strategy α β :=
+  fun _ hist => f_strat g.init_game_state (hist ++ [f_act])
+
+
+lemma zSymm_Game_World.history_reconditioned
+  (g : zSymm_Game_World α β) (f_act : β) (f_act_leg : g.law g.init_game_state [] f_act)
+  (snd_s ws : Strategy α β) :
+  ∀ t : ℕ,
+  History_on_turn g.init_game_state (g.snd_strat_reconditioned ws f_act f_act_leg) snd_s (t+1) =
+  History_on_turn (world_after_fst g f_act f_act_leg).init_game_state (g.fst_strat_reconditioned snd_s f_act) ws (t) ++ [f_act]
+  :=
+  by
+  intro t
+  induction' t with t ih
+  · dsimp [History_on_turn]
+    rw [if_pos (by decide)]
+    dsimp [snd_strat_reconditioned]
+    rw [if_pos (by rfl)]
+  · unfold History_on_turn
+    by_cases q : Turn_fst (t+1+1)
+    · rw [if_pos q]
+      rw [iff_not_comm.mp (Turn_fst_not_step (t+1))] at q
+      rw [if_neg q]
+      dsimp [snd_strat_reconditioned, fst_strat_reconditioned]
+      rw [if_neg (by apply History_on_turn_nonempty_of_succ)]
+      congr
+      rw [ih]
+      rw [List.dropLast_append_of_ne_nil]
+      · dsimp
+        rw [List.append_nil]
+      · apply List.cons_ne_nil
+    · rw [if_neg q]
+      rw [iff_not_comm.mp (Turn_fst_not_step (t+1)), not_not] at q
+      rw [if_pos q]
+      dsimp [snd_strat_reconditioned, fst_strat_reconditioned]
+      congr
+
+
+lemma zSymm_Game_World.snd_reconditioned_legal
+  (g : zSymm_Game_World α β) (f_act : β) (f_act_leg : g.law g.init_game_state [] f_act)
+  (snd_s ws : Strategy α β)
+  (hf : Strategy_legal_fst g.init_game_state g.law (snd_strat_reconditioned ws f_act g f_act_leg) snd_s)
+  : Strategy_legal_snd (world_after_fst g f_act f_act_leg).toSymm_Game_World.init_game_state
+      (world_after_fst g f_act f_act_leg).toSymm_Game_World.law (fst_strat_reconditioned snd_s f_act g) ws
+  :=
+  by
+  intro t ts
+  specialize hf (t+1) (by rw [← Turn_snd_fst_step] ; exact ts)
+  rw [g.history_reconditioned] at hf
+  have := (g.hyper_legal_blind_toStrong g.is_hyper_legal_blind).2
+  dsimp [Symm_Game_World.strong_legal_blind_snd] at this
+  rw [← this] at hf
+  clear this
+  rw [zSymm_Game_World.world_after_fst_law]
+  convert hf using 1
+  · dsimp [snd_strat_reconditioned]
+    rw [if_neg (by apply List.append_ne_nil_of_ne_nil_right ; exact List.cons_ne_nil f_act [])]
+    congr
+    rw [List.dropLast_append_of_ne_nil]
+    · dsimp
+      rw [List.append_nil]
+    · apply List.cons_ne_nil
+  · apply f_act_leg
+
+lemma zSymm_Game_World.snd_reconditioned_legal'
+  (g : zSymm_Game_World α β) (f_act : β) (f_act_leg : g.law g.init_game_state [] f_act)
+  (snd_s ws : Strategy α β)
+  (hf : Strategy_legal_snd (world_after_fst g f_act f_act_leg).toSymm_Game_World.init_game_state
+      (world_after_fst g f_act f_act_leg).toSymm_Game_World.law (fst_strat_reconditioned snd_s f_act g) ws)
+  : Strategy_legal_fst g.init_game_state g.law (snd_strat_reconditioned ws f_act g f_act_leg) snd_s
+  :=
+  by
+  intro t tf
+  cases' t with t
+  · dsimp [History_on_turn, snd_strat_reconditioned]
+    rw [if_pos (by rfl)]
+    exact f_act_leg
+  · specialize hf t (by rw [Turn_snd_fst_step] ; exact tf)
+    rw [g.history_reconditioned]
+    have := (g.hyper_legal_blind_toStrong g.is_hyper_legal_blind).2
+    dsimp [Symm_Game_World.strong_legal_blind_snd] at this
+    rw [← this]
+    clear this
+    rw [zSymm_Game_World.world_after_fst_law] at hf
+    convert hf using 1
+    · dsimp [snd_strat_reconditioned]
+      rw [if_neg (by apply List.append_ne_nil_of_ne_nil_right ; exact List.cons_ne_nil f_act [])]
+      congr
+      rw [List.dropLast_append_of_ne_nil]
+      · dsimp
+        rw [List.append_nil]
+      · apply List.cons_ne_nil
+    · apply f_act_leg
+
+
+
+lemma zSymm_Game_World.fst_reconditioned_legal
+  (g : zSymm_Game_World α β) (f_act : β) (f_act_leg : g.law g.init_game_state [] f_act)
+  (snd_s ws : Strategy α β)
+  (hs : Strategy_legal_snd g.init_game_state g.law (snd_strat_reconditioned ws f_act g f_act_leg) snd_s)
+  : Strategy_legal_fst (world_after_fst g f_act f_act_leg).toSymm_Game_World.init_game_state
+      (world_after_fst g f_act f_act_leg).toSymm_Game_World.law (fst_strat_reconditioned snd_s f_act g) ws
+  :=
+  by
+  intro t ts
+  specialize hs (t+1) (by rw [← Turn_fst_snd_step] ; exact ts)
+  rw [g.history_reconditioned] at hs
+  have := (g.hyper_legal_blind_toStrong g.is_hyper_legal_blind).2
+  dsimp [Symm_Game_World.strong_legal_blind_snd] at this
+  rw [← this] at hs
+  clear this
+  rw [zSymm_Game_World.world_after_fst_law]
+  convert hs using 1
+  apply f_act_leg
+
+
+
+lemma zSymm_Game_World.state_reconditioned
+  (g : zSymm_Game_World α β) (f_act : β) (f_act_leg : g.law g.init_game_state [] f_act)
+  (snd_s ws : Strategy α β) :
+  ∀ t : ℕ,
+  g.state_on_turn (g.snd_strat_reconditioned ws f_act f_act_leg) snd_s (t+1) =
+  (world_after_fst g f_act f_act_leg).state_on_turn (g.fst_strat_reconditioned snd_s f_act) ws (t)
+  :=
+  by
+  intro t
+  cases' t with t
+  · dsimp [Symm_Game_World.state_on_turn, Game_World.history_on_turn, History_on_turn, snd_strat_reconditioned]
+    rw [if_pos (by decide)]
+    rw [if_pos (by rfl)]
+    rfl
+  · dsimp [Symm_Game_World.state_on_turn]
+    by_cases q : Turn_fst (t + 1 + 1)
+    · rw [if_pos q]
+      rw [iff_not_comm.mp (Turn_fst_not_step (t+1))] at q
+      rw [if_neg q]
+      have := careless_singleton _ _ _ _ _ g.transition_careless
+      unfold Symm_Game_World.history_on_turn
+      rw [zSymm_Game_World.history_reconditioned]
+      rw [this]
+      · congr
+        dsimp [snd_strat_reconditioned]
+        rw [if_neg (by apply List.append_ne_nil_of_ne_nil_right ; apply List.cons_ne_nil)]
+        rw [List.dropLast_append_of_ne_nil]
+        · dsimp
+          rw [List.append_nil]
+        · apply List.cons_ne_nil
+      · apply f_act_leg
+    · rw [if_neg q]
+      rw [iff_not_comm.mp (Turn_fst_not_step (t+1)), not_not] at q
+      rw [if_pos q]
+      have := careless_singleton _ _ _ _ _ g.transition_careless
+      unfold Symm_Game_World.history_on_turn
+      rw [zSymm_Game_World.history_reconditioned]
+      rw [this]
+      · congr
+      · apply f_act_leg
+
+
+
+lemma zSymm_Game_World.state_neutral_reconditioned
+  (g : zSymm_Game_World α β) (f_act : β) (f_act_leg : g.law g.init_game_state [] f_act)
+  (snd_s ws : Strategy α β) :
+  ∀ t : ℕ,
+  g.state_on_turn_neutral (g.snd_strat_reconditioned ws f_act f_act_leg) snd_s (t+1) =
+  (world_after_fst g f_act f_act_leg).state_on_turn_neutral (g.fst_strat_reconditioned snd_s f_act) ws (t)
+  :=
+  by
+  intro t
+  unfold Symm_Game_World.state_on_turn_neutral
+  by_cases q : Turn_fst (t + 1)
+  · rw [if_pos q]
+    rw [iff_not_comm.mp (Turn_fst_not_step (t))] at q
+    rw [if_neg q]
+    rw [zSymm_Game_World.world_after_fst_win_states]
+    congr 2
+    apply zSymm_Game_World.state_reconditioned
+  · rw [if_neg q]
+    rw [iff_not_comm.mp (Turn_fst_not_step (t)), not_not] at q
+    rw [if_pos q]
+    rw [zSymm_Game_World.world_after_fst_win_states]
+    congr 2
+    apply zSymm_Game_World.state_reconditioned
+
+
+
+
+
+lemma zSymm_Game_World.reCondition_win
+  (g : zSymm_Game_World α β) (f_act : β) (f_act_leg : g.law g.init_game_state [] f_act)
+  (snd_s ws : Strategy α β)
+  (ws_leg : Strategy_legal_fst g.init_game_state g.law (snd_strat_reconditioned ws f_act g f_act_leg) snd_s)
+  (snd_leg : Strategy_legal_snd g.init_game_state g.law (snd_strat_reconditioned ws f_act g f_act_leg) snd_s)
+  (wlg_ws : ¬Symm_Game_World.win_states g.toSymm_Game_World g.init_game_state)
+  (H : Symm_Game.snd_win
+    { toSymm_Game_World := (g.world_after_fst f_act f_act_leg).toSymm_Game_World,
+      fst_strat := g.fst_strat_reconditioned snd_s f_act,
+      snd_strat := ws,
+      fst_lawful :=
+          (by
+           apply zSymm_Game_World.fst_reconditioned_legal
+           exact snd_leg)
+      snd_lawful :=
+        (by
+           apply zSymm_Game_World.snd_reconditioned_legal
+           exact ws_leg)
+      })
+  : Symm_Game.fst_win
+  { toSymm_Game_World := g.toSymm_Game_World, fst_strat := snd_strat_reconditioned ws f_act g f_act_leg, snd_strat := snd_s,
+    fst_lawful := ws_leg, snd_lawful := snd_leg } :=
+  by
+  obtain ⟨t,ts,tw,tn⟩ := H
+  use (t+1)
+  constructor
+  · rw [← Turn_snd_fst_step]
+    exact ts
+  · constructor
+    · dsimp
+      rw [zSymm_Game_World.world_after_fst_win_states] at tw
+      convert tw using 1
+      apply zSymm_Game_World.state_reconditioned
+    · intro n nt
+      cases' n with n
+      · dsimp [Symm_Game.state_on_turn_neutral]
+        rw [if_neg (by decide)]
+        dsimp [Symm_Game.state_on_turn]
+        exact wlg_ws
+      · have := g.state_neutral_reconditioned
+        apply Symm_Game.state_on_turn_neutral_from_World _ (n+1)
+        dsimp
+        rw [this]
+        apply tn
+        exact Nat.lt_of_add_lt_add_right nt
