Games/gameLib_fix/Zermelo_new.lean
@@ -1,0 +1,178 @@
+
+import Games.gameLib_fix.Termination
+
+
+lemma Game_World.not_has_WL (g : Game_World α β) (h : ¬ g.has_WL) :
+  ¬ g.is_fst_win ∧ ¬ g.is_snd_win :=
+  by
+  contrapose h
+  simp_rw [not_and_or, not_not] at h
+  rw [not_not]
+  cases' h with h h
+  · exact Game_World.has_WL.wf h
+  ·  exact Game_World.has_WL.ws h
+
+
+
+-- variable {α β : Sort _} in -- inside leads to massive problems, fixed from 4.9 onwards
+-- mutual -- Remeber to thank Arthur Adjedj
+-- inductive History_good  (ini : α) (f_law s_law : α → List β → (β → Prop)) (f_trans s_trans : α → List β → (β → α)) (f_wins s_wins : α → Prop) : List β → Prop where
+-- | mk hist : Hist_legal ini f_law s_law (hist) → State_from_history_neutral ini f_trans s_trans f_wins s_wins hist →  auxExists ini f_law s_law f_trans s_trans f_wins s_wins hist  →  History_good ini f_law s_law f_trans s_trans f_wins s_wins hist
+
+-- inductive auxExists (ini : α) (f_law s_law : α → List β → (β → Prop)) (f_trans s_trans : α → List β → (β → α)) (f_wins s_wins : α → Prop) : List β  → Prop where
+-- | intro hist  (next : β)  :  History_good ini f_law s_law f_trans s_trans f_wins s_wins (next :: hist)  → auxExists ini f_law s_law f_trans s_trans f_wins s_wins hist
+-- end
+
+-- noncomputable
+-- def auxExists_choose (ini : α) (f_law s_law : α → List β → (β → Prop)) (f_trans s_trans : α → List β → (β → α)) (f_wins s_wins : α → Prop)
+--   (hist : List β) (main : auxExists ini f_law s_law f_trans s_trans f_wins s_wins hist) :=
+--   Classical.choice <| let ⟨_,x, px⟩ := main; ⟨(⟨x, px⟩ : {next // History_good ini f_law s_law f_trans s_trans f_wins s_wins (next :: hist) })⟩
+
+-- def Game_World.history_good (g : Game_World α β) := History_good g.init_game_state g.fst_legal g.snd_legal g.fst_transition g.snd_transition g.fst_win_states g.snd_win_states
+
+-- def Game_World.aux_exist (g : Game_World α β) := auxExists g.init_game_state g.fst_legal g.snd_legal g.fst_transition g.snd_transition g.fst_win_states g.snd_win_states
+
+-- noncomputable
+-- def Game_World.aux_exist_choose (g : Game_World α β) (hist : List β) (main : g.aux_exist hist) := auxExists_choose g.init_game_state g.fst_legal g.snd_legal g.fst_transition g.snd_transition g.fst_win_states g.snd_win_states hist main
+
+
+-- def Game_World.playable (g : Game_World α β) : Prop := ∀ hist : List β, Hist_legal g.init_game_state g.fst_legal g.snd_legal hist →
+--   --State_from_history_neutral g.init_game_state g.fst_transition g.snd_transition g.fst_win_states g.snd_win_states hist →
+--   (Turn_fst (hist.length+1) → ∃ act : β, g.fst_legal g.init_game_state hist act) ∧ (Turn_snd (hist.length+1) → ∃ act : β, g.snd_legal g.init_game_state hist act)
+
+
+-- -- Assumes that the initial satte is neutral
+-- inductive State_from_history_neutral_strong (ini : α) (f_trans s_trans : α → List β → (β → α)) (f_wins s_wins : α → Prop) : List β → Prop where
+-- | nil : State_from_history_neutral_strong ini f_trans s_trans f_wins s_wins []
+-- | cons (act : β) (hist : List β) : State_from_history_neutral_strong ini f_trans s_trans f_wins s_wins hist →
+--     State_from_history_neutral ini f_trans s_trans f_wins s_wins (act :: hist) → State_from_history_neutral_strong ini f_trans s_trans f_wins s_wins (act :: hist)
+
+
+-- open Classical
+
+-- noncomputable
+-- def damocles_fStrategy (g : Game_World α β) (hg : g.playable) : fStrategy g.init_game_state g.fst_legal g.snd_legal :=
+--   fun (hist : List β)  (T : Turn_fst (hist.length+1)) (leg : Hist_legal g.init_game_state g.fst_legal g.snd_legal hist) =>
+--   if N : ∃ act, g.fst_legal g.init_game_state hist act ∧ g.fst_win_states (State_from_history g.init_game_state g.fst_transition g.snd_transition (act :: hist))
+--   then ⟨Classical.choose N, (Classical.choose_spec N).1⟩
+--   else ⟨Classical.choose ((hg hist leg).1 T) , Classical.choose_spec ((hg hist leg).1 T)⟩
+
+-- noncomputable
+-- def damocles_sStrategy (g : Game_World α β) (hg : g.playable) : sStrategy g.init_game_state g.fst_legal g.snd_legal :=
+--   fun (hist : List β)  (T : Turn_snd (hist.length+1)) (leg : Hist_legal g.init_game_state g.fst_legal g.snd_legal hist) =>
+--   if N : ∃ act, g.snd_legal g.init_game_state hist act ∧ g.snd_win_states (State_from_history g.init_game_state g.fst_transition g.snd_transition (act :: hist))
+--   then ⟨Classical.choose N, (Classical.choose_spec N).1⟩
+--   else ⟨Classical.choose ((hg hist leg).2 T) , Classical.choose_spec ((hg hist leg).2 T)⟩
+
+
+-- structure history_safe (g : Game_World α β) (hist : List β) : Prop where
+--   leg : Hist_legal g.init_game_state g.fst_legal g.snd_legal hist
+--   neu : State_from_history_neutral_strong g.init_game_state g.fst_transition g.snd_transition g.fst_win_states g.snd_win_states hist
+--   prolong_fst : (Turn_fst (hist.length+1) → ∃ act : β, g.fst_legal g.init_game_state hist act ∧ (∀ next : β, g.snd_legal g.init_game_state (act :: hist) next → ¬ g.snd_win_states (State_from_history g.init_game_state g.fst_transition g.snd_transition (next :: act :: hist))))
+--   prolong_snd : (Turn_snd (hist.length+1) → ∃ act : β, g.snd_legal g.init_game_state hist act ∧ (∀ next : β, g.fst_legal g.init_game_state (act :: hist) next → ¬ g.fst_win_states (State_from_history g.init_game_state g.fst_transition g.snd_transition (next :: act :: hist))))
+
+
+def Hist_from_moves (moves : ℕ → β) : ℕ → List β := fun t => ((List.range t).reverse.map moves)
+
+lemma Hist_from_moves_length (moves : ℕ → β) : ∀ t, (Hist_from_moves moves t).length = t := by
+  intro t ; dsimp [Hist_from_moves] ; rw [List.length_map, List.length_reverse, List.length_range]
+
+lemma Hist_from_moves_succ (moves : ℕ → β) : ∀ t, (Hist_from_moves moves (t+1)) = (moves (t)) :: (Hist_from_moves moves (t)):= by
+  intro t ; dsimp [Hist_from_moves] ; rw [List.range_succ, List.reverse_append, List.map_append, List.reverse_singleton, List.map_singleton, List.singleton_append]
+
+
+--#exit
+
+def Game_World.isWL_alt (g : Game_World α β) : Prop :=
+  ∀ moves : ℕ → β, (∀ t, Hist_legal g.init_game_state g.fst_legal g.snd_legal (Hist_from_moves moves t)) →
+    ∃ T, (g.fst_win_states (State_from_history g.init_game_state  g.fst_transition g.snd_transition (Hist_from_moves moves T))) ∨ (g.snd_win_states (State_from_history g.init_game_state  g.fst_transition g.snd_transition (Hist_from_moves moves T)))
+
+lemma Game_World.isWLiff_isWL_alt (g : Game_World α β) : g.isWL ↔ g.isWL_alt :=
+  by
+  constructor
+  · sorry
+  · intro h f_strat s_strat
+    let moves :=
+      fun t =>
+      let H := (History_on_turn g.init_game_state g.fst_legal g.snd_legal f_strat s_strat t)
+      if T : Turn_fst (t+1) then (f_strat H.val (by rw [H.property.2] ; exact T) H.property.1).val else (s_strat H.val (by rw [Turn_snd_iff_not_fst, H.property.2] ; exact T) H.property.1).val
+    specialize h moves _
+    · intro t
+      induction' t with t ih
+      · dsimp [Hist_from_moves]
+        apply Hist_legal.nil
+      · rw [Hist_from_moves_succ]
+        apply Hist_legal.cons _ _ _ ih
+        let H := (Hist_from_moves moves t)
+        split_ifs with T
+        · convert (f_strat H T ih).property
+          dsimp [moves]
+          rw [Hist_from_moves_length] at T
+          simp_rw [dif_pos T]
+
+
+    · sorry
+
+#exit
+
+/-
+Idea:
+
+consider type of histories that are legal and neutral ; nonempty → empty hist ; disjoin on whether the length are bounded
+or unbounded ; in the unbounded case show that the negation of the above `isWL_alt` holds ; in the bounded case, for a bound
+T, show Zermelo by induction on T, as in the classic proof ?
+Maybe look at histories rather then changing game-world. For a given hist, consider the set of hists that extend it and
+reached a terminal state (there must be one such extention, by the case we're in)....
+For inclusion maximal histories, next move must be terminating
+-/
+
+
+variable {α β : Sort _} in -- inside leads to massive problems, fixed from 4.9 onwards
+mutual  -- Remeber to thank Arthur Adjedj
+
+inductive Hist_good_fst (g : Game_World α β) : List β → Prop where
+| ofWin (hist : List β) : Hist_legal g.init_game_state g.fst_legal g.snd_legal hist → Turn_fst (hist.length + 1) → g.fst_win_states (State_from_history g.init_game_state  g.fst_transition g.snd_transition hist) → Hist_good_fst g hist
+| ofFst (hist : List β) : Hist_legal g.init_game_state g.fst_legal g.snd_legal hist → Turn_fst (hist.length + 1) → auxExists_fst g hist → Hist_good_fst g hist
+| ofSnd (hist : List β) : Hist_legal g.init_game_state g.fst_legal g.snd_legal hist → Turn_snd (hist.length + 1) → (∀ next : β, g.snd_legal g.init_game_state hist next →  Hist_good_fst g (next :: hist)) → Hist_good_fst g hist
+
+
+inductive auxExists_fst (g : Game_World α β) : List β → Prop where
+| intro (hist : List β) : (next : β) → g.fst_legal g.init_game_state hist next → Hist_good_fst g (next :: hist) → auxExists_fst g hist
+end
+
+
+variable {α β : Sort _} in -- inside leads to massive problems, fixed from 4.9 onwards
+mutual  -- Remeber to thank Arthur Adjedj
+
+inductive Hist_good_snd (g : Game_World α β) : List β → Prop where
+| ofWin (hist : List β) : Hist_legal g.init_game_state g.fst_legal g.snd_legal hist → Turn_snd (hist.length + 1) → g.fst_win_states (State_from_history g.init_game_state  g.fst_transition g.snd_transition hist) → Hist_good_snd g hist
+| ofSnd (hist : List β) : Hist_legal g.init_game_state g.fst_legal g.snd_legal hist → Turn_snd (hist.length + 1) → auxExists_snd g hist → Hist_good_snd g hist
+| ofFst (hist : List β) : Hist_legal g.init_game_state g.fst_legal g.snd_legal hist → Turn_fst (hist.length + 1) → (∀ next : β, g.fst_legal g.init_game_state hist next →  Hist_good_snd g (next :: hist)) → Hist_good_snd g hist
+
+
+inductive auxExists_snd (g : Game_World α β) : List β → Prop where
+| intro (hist : List β) : (next : β) → g.snd_legal g.init_game_state hist next → Hist_good_snd g (next :: hist) → auxExists_snd g hist
+end
+
+
+noncomputable
+def auxExists_fst_choose (g : Game_World α β) (hist : List β) (main : auxExists_fst (g : Game_World α β) hist) :=
+  Classical.choice <| let ⟨_,x, xl,xg⟩ := main; ⟨(⟨x, ⟨xl,xg⟩⟩ : {next // g.fst_legal g.init_game_state hist next ∧ Hist_good_fst g (next :: hist) })⟩
+
+noncomputable
+def auxExists_snd_choose (g : Game_World α β) (hist : List β) (main : auxExists_snd (g : Game_World α β) hist) :=
+  Classical.choice <| let ⟨_,x, xl,xg⟩ := main; ⟨(⟨x, ⟨xl,xg⟩⟩ : {next // g.snd_legal g.init_game_state hist next ∧ Hist_good_snd g (next :: hist) })⟩
+
+
+
+
+#exit
+
+lemma Game_World.Zermelo (g : Game_World α β) :
+  g.isWL → g.has_WL :=
+  by
+  intro h
+  contrapose h
+  replace h := g.not_has_WL h
+  dsimp [is_fst_win, is_snd_win] at h
+  push_neg at h
